Fix provided chapter05 exercises in chapter06

chapter06-refinement/CommitTypes.dfy
@@ -2,7 +2,11 @@
 module CommitTypes {
   // How a particular participant feels.
   datatype Vote = Yes | No
+
   // What decision has been reached by the protocol.
   datatype Decision = Commit | Abort
-}
 
+  // Define events for this state machine (and the ch6 spec state machine it
+  // refines).
+  datatype Event = ParticipantLearnsEvent(idx: nat) | CoordinatorLearnsEvent() | NoOpEvent()
+}
