chapter06-refinement/exercise01.dfy
@@ -1,6 +1,28 @@
 //#title Two Phase Commit Model
 //#desc Model a distributed protocol using compound state machines.
 
+// This is an instructor-provided solution to chapter 5, with some tweaks to
+// make is suitable for refinement. We've gone through the host and distributed
+// system state machines and added an "event" parameter to all the Next and
+// transition predicates that will be used in the chapter 6 refinement theorems.
+//
+// Each transition now specifies which "event" it is simulating from a more
+// abstract state machine that models two-phase commit. You'll define exactly
+// what those events mean when you define that abstract state machine in
+// ch06exercise01, and in the refinement proof you'll show that when the
+// distributed state machine claims that `event` happened the abstract state
+// machine agrees.
+//
+// The exact events the distributed state machine "emits" (alongside each
+// transition) will probably make more sense when you get to doing the proof; at
+// that point we'd recommend coming back and reading these definitions. You'll
+// notice many steps use the event NoOpEvent. This is because even though the
+// distributed state machine transitioned and made progress, it's claiming to
+// have made no progress in the _abstract_ state machine. For example, sending
+// votes to the coordinator doesn't actually change any decisions until the
+// coordinator receives the last one and processes all of its received votes
+// (which happens in its own Decide step in our solution).
+
 // Your goal is to model a 2-Phase Commit protocol. You're modeling a single
 // instance of the problem -- a designated coordinator, no concurrent
 // instances. Furthermore, you may assume there are no coordinator or
@@ -35,7 +57,6 @@
 
 include "UtilitiesLibrary.dfy"
 include "CommitTypes.dfy"
-//#extract CommitTypes.template solution CommitTypes.dfy
 
 module Types {
   import opened UtilitiesLibrary
@@ -47,11 +68,11 @@ module Types {
   // (There are cleverer ways to parameterize the network module, but
   // we're trying to avoid getting fancy with the Dafny module system.)
   datatype Message =
-/*{*/
+      /*{*/
     | VoteReqMsg                           // from leader
     | VoteMsg(sender: HostId, vote: Vote)  // from participant
     | DecisionMsg(decision: Decision)
-/*}*/
+      /*}*/
 
   // A MessageOps is a "binding variable" used to connect a Host's Next step
   // (what message got received, what got sent?) with the Network (only allow
@@ -72,53 +93,53 @@ module CoordinatorHost {
   import opened Types
   import opened UtilitiesLibrary
 
-/*{*/
+  /*{*/
   datatype Constants = Constants(participantCount: nat)
-/*}*/
+  /*}*/
 
   // What relationship must hold between this host's own constants and the
   // structure of the overall group of hosts? It needs to have a correct
   // count of the number of participants.
   ghost predicate ConstantsValidForGroup(c: Constants, participantCount: nat)
   {
-/*{*/
+    /*{*/
     && c.participantCount == participantCount
-/*}*/
+    /*}*/
   }
 
   datatype Variables = Variables(
     decision: Option<Decision>
-/*{*/
-    ,
+    /*{*/
+  ,
     votes: seq<Option<Vote>>
-/*}*/
+    /*}*/
   )
   {
     // WF is for a simple condition that relates every valid Variables state
     // to the Constants.
     ghost predicate WF(c: Constants) {
-/*{*/
+      /*{*/
       && |votes| == c.participantCount
-/*}*/
+      /*}*/
     }
   }
 
   ghost predicate Init(c: Constants, v: Variables)
   {
-/*{*/
+    /*{*/
     && v.WF(c)
-    // No votes recorded yet
+       // No votes recorded yet
     && (forall hostIdx:HostId | hostIdx < |v.votes| :: v.votes[hostIdx].None?)
-    // No decision recorded yet
+                                                       // No decision recorded yet
     && v.decision.None?
-/*}*/
+       /*}*/
   }
 
   // Protocol steps. Define an action predicate for each step of the protocol
   // that the coordinator is involved in.
   // Hint: it's probably easiest to separate the receipt and recording of
   // incoming votes from detecting that all have arrived and making a decision.
-/*{*/
+  /*{*/
   ghost predicate SendReq(c: Constants, v: Variables, v': Variables, msgOps: MessageOps)
   {
     && v.WF(c)
@@ -135,7 +156,7 @@ module CoordinatorHost {
     && var recvMsg := msgOps.recv.value;
     && recvMsg.VoteMsg?
     && recvMsg.sender < c.participantCount
-    // Record sender's vote.
+       // Record sender's vote.
     && v' == v.(votes := v.votes[recvMsg.sender := Some(recvMsg.vote)])
     && msgOps.send.None?
   }
@@ -151,49 +172,51 @@ module CoordinatorHost {
     && v.WF(c)
     && AllVotesCollected(c, v)
     && decision ==
-      if (forall hostIdx:HostId | hostIdx < |v.votes| :: v.votes[hostIdx].value.Yes?)
-      then Commit
-      else Abort
+       if (forall hostIdx:HostId | hostIdx < |v.votes| :: v.votes[hostIdx].value.Yes?)
+       then Commit
+       else Abort
   }
 
-  ghost predicate Decide(c: Constants, v: Variables, v': Variables, decision: Decision, msgOps: MessageOps)
+  ghost predicate Decide(c: Constants, v: Variables, v': Variables, decision: Decision, event: Event, msgOps: MessageOps)
   {
     && v.WF(c)
     && v'.WF(c)
     && msgOps.recv.None?
+    && (event == if v.decision.None? then CoordinatorLearnsEvent
+                 else NoOpEvent)
     && ObservesResult(c, v, decision)
-    // Record the decision
+       // Record the decision
     && v' == v.(decision := Some(decision))
-    // Transmit the decision
+       // Transmit the decision
     && msgOps.send == Some(DecisionMsg(decision))
   }
-/*}*/
+  /*}*/
 
   // JayNF
   datatype Step =
-/*{*/
+      /*{*/
     | SendReqStep
     | LearnVoteStep
     | DecideStep(decision: Decision)
-/*}*/
+      /*}*/
 
   // msgOps is a "binding variable" -- the host and the network have to agree
   // on its assignment to make a valid transition. So the host explains what
   // would happen if it could receive a particular message, and the network
   // decides whether such a message is available for receipt.
-  ghost predicate NextStep(c: Constants, v: Variables, v': Variables, step: Step, msgOps: MessageOps)
+  ghost predicate NextStep(c: Constants, v: Variables, v': Variables, event: Event, step: Step, msgOps: MessageOps)
   {
     match step
-/*{*/
-      case SendReqStep => SendReq(c, v, v', msgOps)
-      case LearnVoteStep => LearnVote(c, v, v', msgOps)
-      case DecideStep(decision) => Decide(c, v, v', decision, msgOps)
-/*}*/
+    /*{*/
+    case SendReqStep => SendReq(c, v, v', msgOps) && event == NoOpEvent
+    case LearnVoteStep => LearnVote(c, v, v', msgOps) && event == NoOpEvent
+    case DecideStep(decision) => Decide(c, v, v', decision, event, msgOps)
+    /*}*/
   }
 
-  ghost predicate Next(c: Constants, v: Variables, v': Variables, msgOps: MessageOps)
+  ghost predicate Next(c: Constants, v: Variables, v': Variables, event: Event, msgOps: MessageOps)
   {
-    exists step :: NextStep(c, v, v', step, msgOps)
+    exists step :: NextStep(c, v, v', event, step, msgOps)
   }
 }
 
@@ -208,69 +231,72 @@ module ParticipantHost {
   // structure of the overall group of hosts? It needs to know its hostId.
   ghost predicate ConstantsValidForGroup(c: Constants, hostId: HostId)
   {
-/*{*/
+    /*{*/
     && c.hostId == hostId
-/*}*/
+    /*}*/
   }
 
   datatype Variables = Variables(decision: Option<Decision>)
   {
     ghost predicate WF(c: Constants) {
-/*{*/
+      /*{*/
       true
-/*}*/
+      /*}*/
     }
   }
 
   ghost predicate Init(c: Constants, v: Variables)
   {
-/*{*/
+    /*{*/
     && v.decision.None?
-/*}*/
+    /*}*/
   }
 
   // Protocol steps. Define an action predicate for each step of the protocol
   // that participant can take.
-/*{*/
-  ghost predicate Vote(c: Constants, v: Variables, v': Variables, msgOps: MessageOps)
+  /*{*/
+  ghost predicate Vote(c: Constants, v: Variables, v': Variables, event: Event, msgOps: MessageOps)
   {
     && msgOps.recv.Some?
     && var recvMsg := msgOps.recv.value;
     && recvMsg.VoteReqMsg?
     && msgOps.send == Some(VoteMsg(c.hostId, c.preference))
-    // Infer Abort decision if we're voting No
-    && v'.decision == if c.preference.No? then Some(Abort) else v.decision
+       // Infer Abort decision if we're voting No
+    && v'.decision == (if c.preference.No? then Some(Abort) else v.decision)
+       // Take ParticipantLearnEvent step if we made a local decision
+    && event == (if v.decision.None? && v'.decision.Some? then ParticipantLearnsEvent(c.hostId) else NoOpEvent)
   }
 
-  ghost predicate LearnDecision(c: Constants, v: Variables, v': Variables, msgOps: MessageOps)
+  ghost predicate LearnDecision(c: Constants, v: Variables, v': Variables, event: Event, msgOps: MessageOps)
   {
     && msgOps.recv.Some?
     && var recvMsg := msgOps.recv.value;
     && recvMsg.DecisionMsg?
+    && (event == if v.decision.None? then ParticipantLearnsEvent(c.hostId) else NoOpEvent)
     && v'.decision == Some(recvMsg.decision)
     && msgOps.send.None?
   }
-/*}*/
+  /*}*/
 
   // JayNF
   datatype Step =
-/*{*/
+      /*{*/
     | VoteStep
     | LearnDecisionStep
-/*}*/
+      /*}*/
 
-  ghost predicate NextStep(c: Constants, v: Variables, v': Variables, step: Step, msgOps: MessageOps)
+  ghost predicate NextStep(c: Constants, v: Variables, v': Variables, event: Event, step: Step, msgOps: MessageOps)
   {
     match step
-/*{*/
-      case VoteStep => Vote(c, v, v', msgOps)
-      case LearnDecisionStep => LearnDecision(c, v, v', msgOps)
-/*}*/
+    /*{*/
+    case VoteStep => Vote(c, v, v', event, msgOps)
+    case LearnDecisionStep => LearnDecision(c, v, v', event, msgOps)
+    /*}*/
   }
 
-  ghost predicate Next(c: Constants, v: Variables, v': Variables, msgOps: MessageOps)
+  ghost predicate Next(c: Constants, v: Variables, v': Variables, event: Event, msgOps: MessageOps)
   {
-    exists step :: NextStep(c, v, v', step, msgOps)
+    exists step :: NextStep(c, v, v', event, step, msgOps)
   }
 }
 
@@ -296,10 +322,10 @@ module Host {
   {
     ghost predicate WF(c: Constants) {
       && (CoordinatorVariables? <==> c.CoordinatorConstants?) // types of c & v agree
-      // subtype WF satisfied
+         // subtype WF satisfied
       && (match c
-            case CoordinatorConstants(_) => coordinator.WF(c.coordinator)
-            case ParticipantConstants(_) => participant.WF(c.participant)
+          case CoordinatorConstants(_) => coordinator.WF(c.coordinator)
+          case ParticipantConstants(_) => participant.WF(c.participant)
           )
     }
   }
@@ -311,25 +337,25 @@ module Host {
   {
     // There must at least be a coordinator
     && 0 < |grp_c|
-    // Last host is a coordinator
+       // Last host is a coordinator
     && Last(grp_c).CoordinatorConstants?
-    // All the others are participants
+       // All the others are participants
     && (forall hostid:HostId | hostid < |grp_c|-1 :: grp_c[hostid].ParticipantConstants?)
-    // The coordinator's constants must correctly account for the number of participants
+                                                     // The coordinator's constants must correctly account for the number of participants
     && CoordinatorHost.ConstantsValidForGroup(Last(grp_c).coordinator, |grp_c|-1)
-    // The participants's constants must match their group positions.
-    // (Actually, they just need to be distinct from one another so we get
-    // non-conflicting votes, but this is an easy way to express that property.)
+       // The participants's constants must match their group positions.
+       // (Actually, they just need to be distinct from one another so we get
+       // non-conflicting votes, but this is an easy way to express that property.)
     && (forall hostid:HostId | hostid < |grp_c|-1
-        :: ParticipantHost.ConstantsValidForGroup(grp_c[hostid].participant, hostid))
+         :: ParticipantHost.ConstantsValidForGroup(grp_c[hostid].participant, hostid))
   }
 
   ghost predicate GroupWF(grp_c: seq<Constants>, grp_v: seq<Variables>)
   {
     && GroupWFConstants(grp_c)
-    // Variables size matches group size defined by grp_c
+       // Variables size matches group size defined by grp_c
     && |grp_v| == |grp_c|
-    // Each host is well-formed
+       // Each host is well-formed
     && (forall hostid:HostId | hostid < |grp_c| :: grp_v[hostid].WF(grp_c[hostid]))
   }
 
@@ -342,23 +368,23 @@ module Host {
   {
     // constants & variables are well-formed (same number of host slots as constants expect)
     && GroupWF(grp_c, grp_v)
-    // Coordinator is initialized to know about the N-1 participants.
+       // Coordinator is initialized to know about the N-1 participants.
     && CoordinatorHost.Init(Last(grp_c).coordinator, Last(grp_v).coordinator)
-    // Participants initted with their ids.
+       // Participants initted with their ids.
     && (forall hostid:HostId | hostid < |grp_c|-1 ::
-        ParticipantHost.Init(grp_c[hostid].participant, grp_v[hostid].participant)
-      )
+         ParticipantHost.Init(grp_c[hostid].participant, grp_v[hostid].participant)
+         )
   }
 
   // Dispatch Next to appropriate underlying implementation.
-  ghost predicate Next(c: Constants, v: Variables, v': Variables, msgOps: MessageOps)
+  ghost predicate Next(c: Constants, v: Variables, v': Variables, event: Event, msgOps: MessageOps)
   {
     && v.WF(c)
     && v'.WF(c)
     && (match c
-      case CoordinatorConstants(_) => CoordinatorHost.Next(c.coordinator, v.coordinator, v'.coordinator, msgOps)
-      case ParticipantConstants(_) => ParticipantHost.Next(c.participant, v.participant, v'.participant, msgOps)
-      )
+        case CoordinatorConstants(_) => CoordinatorHost.Next(c.coordinator, v.coordinator, v'.coordinator, event, msgOps)
+        case ParticipantConstants(_) => ParticipantHost.Next(c.participant, v.participant, v'.participant, event, msgOps)
+        )
   }
 }
 
@@ -389,9 +415,9 @@ module Network {
   {
     // Only allow receipt of a message if we've seen it has been sent.
     && (msgOps.recv.Some? ==> msgOps.recv.value in v.sentMsgs)
-    // Record the sent message, if there was one.
+       // Record the sent message, if there was one.
     && v'.sentMsgs ==
-      v.sentMsgs + if msgOps.send.None? then {} else { msgOps.send.value }
+       v.sentMsgs + if msgOps.send.None? then {} else { msgOps.send.value }
   }
 }
 
@@ -439,13 +465,13 @@ module DistributedSystem {
     && Network.Init(c.network, v.network)
   }
 
-  ghost predicate HostAction(c: Constants, v: Variables, v': Variables, hostid: HostId, msgOps: MessageOps)
+  ghost predicate HostAction(c: Constants, v: Variables, v': Variables, hostid: HostId, event: Event, msgOps: MessageOps)
   {
     && v.WF(c)
     && v'.WF(c)
     && c.ValidHostId(hostid)
-    && Host.Next(c.hosts[hostid], v.hosts[hostid], v'.hosts[hostid], msgOps)
-    // all other hosts UNCHANGED
+    && Host.Next(c.hosts[hostid], v.hosts[hostid], v'.hosts[hostid], event, msgOps)
+       // all other hosts UNCHANGED
     && (forall otherHost:nat | c.ValidHostId(otherHost) && otherHost != hostid :: v'.hosts[otherHost] == v.hosts[otherHost])
   }
 
@@ -453,40 +479,41 @@ module DistributedSystem {
   datatype Step =
     | HostActionStep(hostid: HostId, msgOps: MessageOps)
 
-  ghost predicate NextStep(c: Constants, v: Variables, v': Variables, step: Step)
+  ghost predicate NextStep(c: Constants, v: Variables, v': Variables, event: Event, step: Step)
   {
-    && HostAction(c, v, v', step.hostid, step.msgOps)
-    // network agrees recv has been sent and records sent
+    && HostAction(c, v, v', step.hostid, event, step.msgOps)
+       // network agrees recv has been sent and records sent
     && Network.Next(c.network, v.network, v'.network, step.msgOps)
   }
 
-  ghost predicate Next(c: Constants, v: Variables, v': Variables)
+  ghost predicate Next(c: Constants, v: Variables, v': Variables, event: Event)
   {
-    exists step :: NextStep(c, v, v', step)
+    exists step :: NextStep(c, v, v', event, step)
   }
 
   ghost function GetDecisionForHost(hv: Host.Variables) : Option<Decision>
   {
     match hv
-      case CoordinatorVariables(coordinator) => coordinator.decision
-      case ParticipantVariables(participant) => participant.decision
+    case CoordinatorVariables(coordinator) => coordinator.decision
+    case ParticipantVariables(participant) => participant.decision
   }
 
   // Convince us that your model does something
-  lemma PseudoLiveness(c: Constants) returns (behavior: seq<Variables>)
+  lemma PseudoLiveness(c: Constants) returns (behavior: seq<Variables>, events: seq<Event>)
     requires c.WF()
     requires |c.hosts| == 2 // There's exactly one voting participant...
     requires c.hosts[0].participant.preference.Yes? // ... who wants a Yes.
     // Exhibit a behavior that satisfies your state machine...
     ensures 0 < |behavior|
+    ensures |events| == |behavior|-1
     ensures Init(c, behavior[0])
-    ensures forall i:nat | i < |behavior|-1 :: Next(c, behavior[i], behavior[i+1])
+    ensures forall i:nat | i < |behavior|-1 :: Next(c, behavior[i], behavior[i+1], events[i])
     // ...and all the participants arrive at a decision.
     ensures Last(behavior).WF(c)
     ensures forall hostid:HostId | c.ValidHostId(hostid)
-      :: GetDecisionForHost(Last(behavior).hosts[hostid]) == Some(Commit)
+              :: GetDecisionForHost(Last(behavior).hosts[hostid]) == Some(Commit)
   {
-/*{*/
+    /*{*/
     var v0 := Variables(
       [
         Host.ParticipantVariables(ParticipantHost.Variables(None)),
@@ -501,8 +528,8 @@ module DistributedSystem {
       ], Network.Variables({VoteReqMsg}));
 
     var mops1 := MessageOps(None, Some(VoteReqMsg));
-    assert CoordinatorHost.NextStep(c.hosts[1].coordinator, v0.hosts[1].coordinator, v1.hosts[1].coordinator, CoordinatorHost.SendReqStep, mops1);
-    assert NextStep(c, v0, v1, HostActionStep(1, mops1));
+    assert CoordinatorHost.NextStep(c.hosts[1].coordinator, v0.hosts[1].coordinator, v1.hosts[1].coordinator, NoOpEvent, CoordinatorHost.SendReqStep, mops1);
+    assert NextStep(c, v0, v1, NoOpEvent, HostActionStep(1, mops1));
 
     var v2 := Variables(
       [
@@ -511,8 +538,8 @@ module DistributedSystem {
       ], Network.Variables({VoteReqMsg, VoteMsg(0, Yes)}));
 
     var mops2 := MessageOps(Some(VoteReqMsg), Some(VoteMsg(0, Yes)));
-    assert ParticipantHost.NextStep(c.hosts[0].participant, v1.hosts[0].participant, v2.hosts[0].participant, ParticipantHost.VoteStep, mops2);
-    assert NextStep(c, v1, v2, HostActionStep(0, mops2));
+    assert ParticipantHost.NextStep(c.hosts[0].participant, v1.hosts[0].participant, v2.hosts[0].participant, NoOpEvent, ParticipantHost.VoteStep, mops2);
+    assert NextStep(c, v1, v2, NoOpEvent, HostActionStep(0, mops2));
 
     var v3 := Variables(
       [
@@ -521,8 +548,8 @@ module DistributedSystem {
       ], Network.Variables({VoteReqMsg, VoteMsg(0, Yes)}));
 
     var mops3 := MessageOps(Some(VoteMsg(0, Yes)), None);
-    assert CoordinatorHost.NextStep(c.hosts[1].coordinator, v2.hosts[1].coordinator, v3.hosts[1].coordinator, CoordinatorHost.LearnVoteStep, mops3);
-    assert NextStep(c, v2, v3, HostActionStep(1, mops3));
+    assert CoordinatorHost.NextStep(c.hosts[1].coordinator, v2.hosts[1].coordinator, v3.hosts[1].coordinator, NoOpEvent, CoordinatorHost.LearnVoteStep, mops3);
+    assert NextStep(c, v2, v3, NoOpEvent, HostActionStep(1, mops3));
 
     var v4 := Variables(
       [
@@ -531,8 +558,8 @@ module DistributedSystem {
       ], Network.Variables({VoteReqMsg, VoteMsg(0, Yes), DecisionMsg(Commit)}));
 
     var mops4 := MessageOps(None, Some(DecisionMsg(Commit)));
-    assert CoordinatorHost.NextStep(c.hosts[1].coordinator, v3.hosts[1].coordinator, v4.hosts[1].coordinator, CoordinatorHost.DecideStep(Commit), mops4);
-    assert NextStep(c, v3, v4, HostActionStep(1, mops4));
+    assert CoordinatorHost.NextStep(c.hosts[1].coordinator, v3.hosts[1].coordinator, v4.hosts[1].coordinator, CoordinatorLearnsEvent, CoordinatorHost.DecideStep(Commit), mops4);
+    assert NextStep(c, v3, v4, CoordinatorLearnsEvent, HostActionStep(1, mops4));
 
     var v5 := Variables(
       [
@@ -541,12 +568,11 @@ module DistributedSystem {
       ], Network.Variables({VoteReqMsg, VoteMsg(0, Yes), DecisionMsg(Commit)}));
 
     var mops5 := MessageOps(Some(DecisionMsg(Commit)), None);
-    assert ParticipantHost.NextStep(c.hosts[0].participant, v4.hosts[0].participant, v5.hosts[0].participant, ParticipantHost.LearnDecisionStep, mops5);
-    assert NextStep(c, v4, v5, HostActionStep(0, mops5));
+    assert ParticipantHost.NextStep(c.hosts[0].participant, v4.hosts[0].participant, v5.hosts[0].participant, ParticipantLearnsEvent(0), ParticipantHost.LearnDecisionStep, mops5);
+    assert NextStep(c, v4, v5, ParticipantLearnsEvent(0), HostActionStep(0, mops5));
 
+    events := [NoOpEvent, NoOpEvent, NoOpEvent, CoordinatorLearnsEvent, ParticipantLearnsEvent(0)];
     behavior := [v0, v1, v2, v3, v4, v5];
-/*}*/
+    /*}*/
   }
 }
-
-
